\[ x^2 - 2xy + z^2 = \sin{x} + y \]
\[ x^2 + y^2 + \frac{z^2}{4} = 8 \]
\[ x + \sin{y} + z^2 = 1 \]
\[ \cos^2{x} + \sin{y} = \tan{z} \]
\[ xy^2 - 2\sin{z} + 1 = x \]
\[ e^{xy} - 5y + 4z^2 = 1 \]
\[ \sin{xz} + z = 3y^2 \]
\[ z = \frac{1}{2} \ln{(x^2+y^2)} \]
\[ \frac{1}{x} + \frac{1}{y} = \frac{1}{z} \]
\[ xe^y - \sqrt{1+z} = 1 \]
\[ z^2 - 1 = \sqrt{x+y+1} \]
\[ \frac{1}{z} - \sin{x} = \frac{1}{\sqrt{4-y^2}} \]
\[ \sin{xy} + \sin{xz} = \sin{yz} \]
\[ \frac{1 + \sin{x}}{e^y} - \frac{1}{z^2 - 1} = 0 \]
\[ x^2 - 2\sin{y} + z^2 = 1 \]
\[ \frac{1}{x} + \frac{x}{y} = \ln{z} \]
\[ \ln{xy} = 2z + 3 \]
\[ e^{x + 4} - \frac{1}{3y-2} = z^2 - 1 \]
\[ \cos{x^2} - \sin^2{y} = z \]
\[ \frac{2}{1 + \cos{2x}} - \frac{1 - \cos{2y}}{2} = z \]
\[ e^y \sin^2{x} = 1 - \sqrt{z} \]
\[ z^2 + 2xyz = x^2 - 4y + 2 \]
\[ x^2 + y^2 - z^2 = 1 \]
\[ \tan{x} - \tan{y} = \sqrt{1 - \frac{1}{z}} \]
\[ x^2 \sqrt{z} + y = 1 \]
\[ \sin{x} + \sin{z} = \frac{1}{2 + y^2} \]
\[ \frac{1}{1+y^2} = \frac{1}{x+z} - 1 \]
\[ x^2 + y^2 + z^2 = 2(xy + xz + yz) + 4 \]
\[ \sin{\frac{x}{2}} = \frac{x}{\sin{y}} - z^2 \]
\[ \ln{x} + 2\ln{y} = z^4 - 1 \]
\[ \sqrt{x+4y} - \frac{1}{y} = \tan{z} \]
\[ \ln{\cos{x}} - 5y^2 = e^z + 3x^2 \]
\[ \cot{\frac{y}{x}} - y = z^2 + \sqrt{2 - x} \]
\[ x^4 + y^4 = 2xy + z^4 - 1 \]
\[ z^2 - x^2 = \sin{xy} \]
\[ y^2 \cos{x} + x^2 = \frac{1}{z+1} \]
\[ \sqrt{x^2 - y^2} = \sin{x} \cdot \sin{z} + 1 \]
\[ \ln\left( x + e^{y} \right) = \frac{2}{\ln{z}} - 1 \]
\[ \sqrt{\frac{x}{\pi} + 1} = z + \sqrt[3]{2 - y} + \sin{x} \]
\[ \sqrt{1 - \frac{xz}{2}} = \cot{y} + \tan{z^2} \]
\[ \frac{1}{\sqrt{1 - x^2}} = x^2 - \frac{z}{xy} \]
\[ x^2 e^y \sin{z} = x^2 - 4xy + 4z^2 \]
\[ x \cos{x} - y \sin{y} = z^2 - 1 \]
\[ \ln{\tan{x}} = y + z^2 \]
\[ \frac{1}{x} + \frac{\ln{z}}{y} = 1 - \sin{x} \]
\[ \frac{1}{\cos{x} + 1} = \frac{z - 1}{\sin{y} - 1} + 2 \]
\[ y\sin{x} = xyz - 4 \]
\[ \sin{x}\sin{y} + \cos{y}\cos{z} = xz \]
\[ \frac{\sin{x}}{\cos{x} + 1} - \frac{\cos{y}}{2} = \sqrt{z} \]
\[ z\tan{xy} = x + y + z \]
\[ e^{x+y+z} = xyz + 1 \]
\[ e^{\cos{x}} = z^2\sin{y} \]
\[ x^4 + y^4 + z^4 = 8xyz \]
\[ \arctan{x} + y = 2\tan{z} \]
\[ e^{\sqrt{x}} = \sqrt{x + 2y - z} \]
\[ (x + y + z)^3 - 2xy = e^z \]
\[ x + 2xy^2 - 3z = \ln(x+z) \]
\[ \tan\left( x^2 + y^2 \right) = \frac{1}{z^2+1} \]
\[ \frac{x+y}{z} - \frac{z-y}{x} = x+1 \]
\[ \arctan{x} + \frac{z}{1+y^2} = \sin{z} \]