\[ x^2 - 2xy + z^2 = \sin{x} + \cos{y}, ~ P = \left( \pi, \frac{\pi}{2}, 0 \right) \]
\[ x^2 + y^2 + \frac{z^2}{4} = 5, ~ P = \left( \sqrt{3}, -1, 2 \right) \]
\[ x - \sin{y} + z^2 = 1, ~ P = \left( -2, \frac{\pi}{2}, 2 \right) \]
\[ \cos^2{x} + 2\sin{y} = \tan{z}, ~ P = \left( \frac{\pi}{2}, \frac{\pi}{3}, \frac{\pi}{3} \right) \]
\[ xy^2 - 2\sin{z} + 1 = x, ~ P = \left( 2, \frac{1}{\sqrt{2}}, \pi \right) \]
\[ e^{xy} - 5y + 4z^2 = 1, ~ P = \left( \ln{2}, 1, 2 \right) \]
\[ \sin{xz} + 4z = 3y^2, ~ P = \left( \pi, -1, \frac{1}{2} \right) \]
\[ z = \frac{1}{2} \ln{(x^2+y^2)}, ~ P = \left( \frac{e}{\sqrt{2}}, -\frac{e}{\sqrt{2}} , 1 \right) \]
\[ \frac{1}{x} + \frac{1}{y} = \frac{1}{z}, ~ P = \left( 2, -3, 6 \right) \]
\[ xe^y - \sqrt{1+z} = 1, ~ P = \left( 1, \ln{3}, 3 \right) \]
\[ z^2 - 1 = \sqrt{x+y+1}, ~ P = \left( 4, 4, 2 \right) \]
\[ \frac{1}{z} - \sin{x} = \frac{1}{\sqrt{4-y^2}}, ~ P = \left( \pi, 0, 2 \right) \]
\[ \sin{xy} + \sin{xz} = \sin{yz}, ~ P = \left( 0, 2, \frac{\pi}{2} \right) \]
\[ \frac{1 + \sin{x}}{e^y} - \frac{1}{z^2 - 1} = 0, ~ P = \left( \pi, 0, \sqrt{2} \right) \]
\[ x^2 - 2\sin{y} + z^2 = 1, ~ P = \left( 1, \frac{\pi}{6}, 1 \right) \]
\[ \frac{1}{x} + \frac{x}{y} = \ln{z}, ~ P = \left( 2, -6, \sqrt[6]{e} \right) \]
\[ \ln{xy} = 2z^2 + 3, ~ P = \left( e^2, e^3, 1 \right) \]
\[ e^{x + 4} - \frac{1}{3y-2} = z^2 - 1, ~ P = \left( -2, 1, e \right) \]
\[ \cos{x^2} - \sin^2{y} = z, ~ P = \left( \sqrt{\pi}, 0, -1 \right) \]
\[ \frac{2}{1 + \cos{2x}} - \frac{1 - \cos{2y}}{2} = z, ~ P = \left( \pi, \frac{\pi}{2}, 0 \right) \]
\[ e^y \sin^2{x} = 1 + \sqrt{z-1}, ~ P = \left( \frac{3\pi}{2}, \ln{2}, 2 \right) \]
\[ z^2 + 2xyz = x^2 - 4y + 2, ~ P = \left( \pi, 0, \sqrt{2} \right) \]
\[ x^2 + y^2 - z^2 = 1, ~ P = \left( 1, \sqrt{2}, \sqrt{2} \right) \]
\[ \tan{x} - \tan{y} = \sqrt{1 - \frac{1}{z}}, ~ P = \left( 0, 0, 1 \right) \]
\[ x^2 \sqrt{z} + y = 1, ~ P = \left( \sqrt{2}, -1, 1 \right) \]
\[ \cos{x} + \sin{z} = \frac{1}{2 + y^2}, ~ P = \left( \frac{\pi}{3}, 0, 0 \right) \]
\[ \frac{1}{1+y^2} = \frac{1}{x+z} + 1, ~ P = \left( -1, 1, -1 \right) \]
\[ x^2 + y^2 + z^2 = 2(xy + xz + yz) + 4, ~ P = \left( 0, 0, 2 \right) \]
\[ \sin{\frac{x}{2}} = \frac{x}{\sin{y}} - z^2 + 1, ~ P = \left( \pi, \frac{\pi}{2}, \sqrt{\pi} \right) \]
\[ \ln{x} + 2\ln{y} = z^4 - 1, ~ P = \left( e, e, \sqrt{2} \right) \]
\[ \sqrt{x+4y} - \frac{1}{y} = \tan{z}, ~ P = \left( 0, 1, \frac{\pi}{4} \right) \]
\[ \ln{\cos{x}} + 5y^2 = 2e^z - 3x^2 + 1, ~ P = \left( 0, 1, \ln{2} \right) \]
\[ \cot{\frac{y}{x}} - 1 = z^2 - 2\sqrt{2 - x}, ~ P = \left( 1, \frac{\pi}{4}, \sqrt{2} \right) \]
\[ x^4 + y^4 = 2xy + z^4 - 1, ~ P = \left( 1, 1, 1 \right) \]
\[ z^2 - x^2 = \sin{xy}, ~ P = \left( 1, \pi, 1 \right) \]
\[ y^2 \cos{x} + x^2 = \frac{1}{z+1}, ~ P = \left( 0, 1, 0 \right) \]
\[ \sqrt{4x^2 - y} = z\sin{x} + 1, ~ P = \left( \frac{\pi}{2}, \pi^2, -1 \right) \]
\[ \ln\left( x + e^{y} \right) = \frac{2}{\ln{z}} - 1, ~ P = \left( 0, 1, e \right) \]
\[ \sqrt{\frac{x}{\pi} + 3} = yz + \sin{x}, ~ P = \left( \pi, 2, 1 \right) \]
\[ \sqrt{1 - \frac{xz}{2}} = \cot{y} + \tan{z^2}, ~ P = \left( e, \frac{\pi}{4}, 0 \right) \]
\[ \frac{1}{\sqrt{1 - x^2}} = x^2 - \frac{z}{y}, ~ P = \left( 0, 1, -1 \right) \]
\[ x^2 e^y \sin{z} = x^3 - 4xy + 4z^2, ~ P = \left( 2, 1, 0 \right) \]
\[ x \cos{x} - y \sin{y} = z^2 - 1, ~ P = \left( 0, 0, 1 \right) \]
\[ \ln{\tan{x}} = y + z^2, ~ P = \left( \frac{\pi}{4}, -2, \sqrt{2} \right) \]
\[ \frac{1}{x} + \frac{\ln{z}}{y} = 1 - \sin{x}, ~ P = \left( \frac{\pi}{2}, \frac{\pi}{2}, \frac{1}{e} \right) \]
\[ \frac{1}{\cos{x} + 1} = \frac{z + 1}{\sin{y} - 1} + 2, ~ P = \left( \frac{\pi}{2}, \pi, 0 \right) \]
\[ y\sin{x} = xyz - 4, ~ P = \left( -\frac{\pi}{2}, 4, 0 \right) \]
\[ y\sin{x} + z\cos{y} = xz, ~ P = \left( 0, \frac{\pi}{2}, 1 \right) \]
\[ \frac{\sin{x}}{\cos{x} + 1} - \frac{\cos{y}}{2} = \sqrt{z}, ~ P = \left( \frac{\pi}{2}, \frac{\pi}{2}, 1 \right) \]
\[ z\tan{xy} = x + y + z - 1, ~ P = \left( 0, 0, 1 \right) \]
\[ e^{x+y+z} = xyz + 4, ~ P = \left( \ln{2}, \ln{2}, 0 \right) \]
\[ e^{\cos{x}} = z^2\sin{y}, ~ P = \left( -\frac{\pi}{2}, \frac{\pi}{2}, 1 \right) \]
\[ x^3 - y^3 - z^3 = 3xyz, ~ P = \left( 2, 1, 1 \right) \]
\[ \arctan{x} + y = 2\tan{z}, ~ P = \left( 1, -\frac{\pi}{4}, 0 \right) \]
\[ e^{\sqrt{x}} = \sqrt{x + 2y - z^2}, ~ P = \left( \ln^2 {2}, 2, \ln{2} \right) \]
\[ (x + y + z)^3 - 2xy = 3e^{z-1}, ~ P = \left( 1, -1, 1 \right) \]
\[ x + 2xy^2 - 3z = \ln(x+z), ~ P = \left( 3, 0, 1 \right) \]
\[ \tan\left( x^2 + y^2 \right) = \frac{1}{z^2+1}, ~ P = \left( \frac{\sqrt{\pi}}{2}, 0, 0 \right) \]
\[ \frac{x+y}{z} - \frac{z-y}{x} = x+1, ~ P = \left( 1, 1, 1 \right) \]
\[ \arctan{x} + \frac{z}{1+y^2} = \sin{z}, ~ P = \left( 0, 1, 0 \right) \]